Weidenbach_Book/IsaSAT.thy
@@ -22,7 +22,7 @@ definition SAT :: \<open>nat clauses \<Rightarrow> nat cdcl\<^sub>W_restart_mset
   \<open>SAT CS = do{
     let T = init_state CS;
     SPEC (\<lambda>U. full cdcl\<^sub>W_restart_mset.cdcl\<^sub>W_stgy T U \<or>
-         (CS \<noteq> {#} \<and> conflicting U \<noteq> None \<and> count_decided (trail U) = 0 \<and>
+          (CS \<noteq> {#} \<and> conflicting U \<noteq> None \<and> count_decided (trail U) = 0 \<and>
           unsatisfiable (set_mset CS)))
   }\<close>
 
