Weidenbach_Book/IsaSAT_Conflict_Analysis.thy
@@ -9,7 +9,7 @@ begin
 
 
 definition get_conflict_wll_is_Nil_heur :: \<open>twl_st_wl_heur \<Rightarrow> bool nres\<close> where
-  \<open>get_conflict_wll_is_Nil_heur = (\<lambda>(M, N, U, D, Q, W, _).
+  \<open>get_conflict_wll_is_Nil_heur = (\<lambda>(M, N, D, Q, W, _).
    do {
      if is_None D
      then RETURN False
